Impl/StateModel.i.dfy
@@ -1,20 +1,21 @@
-include "../PivotBetree/PivotBetreeSpec.i.dfy"
-include "../lib/Base/Message.i.dfy"
-include "../ByteBlockCacheSystem/AsyncDiskModel.s.dfy"
-include "../lib/Base/Option.s.dfy"
-include "../BlockCacheSystem/BetreeCache.i.dfy"
-include "../lib/Lang/NativeTypes.s.dfy"
-include "../lib/DataStructures/LruModel.i.dfy"
-include "../lib/DataStructures/MutableMapModel.i.dfy"
-include "../lib/DataStructures/BitmapModel.i.dfy"
-include "BlockAllocatorModel.i.dfy"
-include "IndirectionTableModel.i.dfy"
-include "CommitterModel.i.dfy"
-include "../BlockCacheSystem/BlockJournalDisk.i.dfy"
-include "../BlockCacheSystem/BlockJournalCache.i.dfy"
-include "../ByteBlockCacheSystem/ByteCache.i.dfy"
-include "DiskOpModel.i.dfy"
-include "StateSectorModel.i.dfy"
+// include "../PivotBetree/PivotBetreeSpec.i.dfy"
+// include "../lib/Base/Message.i.dfy"
+// include "../ByteBlockCacheSystem/AsyncDiskModel.s.dfy"
+// include "../lib/Base/Option.s.dfy"
+// include "../BlockCacheSystem/BetreeCache.i.dfy"
+// include "../lib/Lang/NativeTypes.s.dfy"
+// include "../lib/DataStructures/LruModel.i.dfy"
+// include "../lib/DataStructures/MutableMapModel.i.dfy"
+// include "../lib/DataStructures/BitmapModel.i.dfy"
+// include "BlockAllocatorModel.i.dfy"
+// include "IndirectionTableModel.i.dfy"
+// include "CommitterModel.i.dfy"
+// include "../BlockCacheSystem/BlockJournalDisk.i.dfy"
+// include "../BlockCacheSystem/BlockJournalCache.i.dfy"
+// include "../ByteBlockCacheSystem/ByteCache.i.dfy"
+// include "DiskOpModel.i.dfy"
+include "CommitterImpl.i.dfy"
+include "StateBCModel.i.dfy"
 //
 // This file represents immutability's last stand.
 // It is the highest-fidelity representation of the implementation
@@ -26,198 +27,46 @@ include "StateSectorModel.i.dfy"
 //
 
 module StateModel {
-  import opened Options
-  import opened Sequences
-  import opened NativeTypes
+  // import opened Options
+  // import opened Sequences
+  // import opened NativeTypes
 
-  import BT = PivotBetreeSpec`Internal
-  import Messages = ValueMessage
-  import MS = MapSpec
-  import Pivots = BoundedPivotsLib
-  import BC = BlockCache
-  import JC = JournalCache
-  import BBC = BetreeCache
-  import BJD = BlockJournalDisk
-  import BJC = BlockJournalCache
-  import D = AsyncDisk
-  import M = ByteCache
-  import opened BucketsLib
-  import opened BucketWeights
-  import opened Bounds
-  import LruModel
-  import BitmapModel
-  import UI
-  import MutableMapModel
-  import BlockAllocatorModel
-  import IndirectionTableModel
-  import SectorType
-  import DiskLayout
-  import CommitterModel
-  import opened DiskOpModel
+  // // import BT = PivotBetreeSpec`Internal
+  // import Messages = ValueMessage
+  // import MS = MapSpec
+  // import Pivots = BoundedPivotsLib
+  // // import BC = BlockCache
+  // import JC = JournalCache
+  // // import BBC = BetreeCache
+  // // import BJD = BlockJournalDisk
+  // import BJC = BlockJournalCache
+  // import D = AsyncDisk
+  // import M = ByteCache
+  // import opened BucketsLib
+  // import opened BucketWeights
+  // import opened Bounds
+  // // import LruModel
+  // // import BitmapModel
+  // import UI
+  // import MutableMapModel
+  // // import BlockAllocatorModel
+  // // import IndirectionTableModel
+  // import SectorType
+  // // import DiskLayout
+  // import CommitterModel
+  // import opened DiskOpModel
 
-  import ReferenceType`Internal
-  import SSM = StateSectorModel
+  // import ReferenceType`Internal
+
+  import opened CommitterImpl
+  import StateBCModel
 
   // type Node = BT.G.Node  
-  type Reference = BT.G.Reference
-  type DiskOp = BJD.DiskOp
-  type IndirectionTable = SSM.IndirectionTable
-  type Node = SSM.Node
-  type Sector = SSM.Sector
-
   // type IndirectionTable = IndirectionTableModel.IndirectionTable
-  datatype BCVariables =
-    | Ready(
-        persistentIndirectionTable: IndirectionTable, // this lets us keep track of available LBAs
-                                                         // TODO replace with something that only tracks LBAs
-        frozenIndirectionTable: Option<IndirectionTable>,
-        ephemeralIndirectionTable: IndirectionTable,
-        persistentIndirectionTableLoc: DiskLayout.Location,
-        frozenIndirectionTableLoc: Option<DiskLayout.Location>,
-        outstandingIndirectionTableWrite: Option<BC.ReqId>,
-        outstandingBlockWrites: map<BC.ReqId, BC.OutstandingWrite>,
-        outstandingBlockReads: map<BC.ReqId, BC.OutstandingRead>,
-        cache: map<Reference, Node>,
-        lru: LruModel.LruQueue,
-        blockAllocator: BlockAllocatorModel.BlockAllocatorModel
-      )
-    | LoadingIndirectionTable(
-        indirectionTableLoc: DiskLayout.Location,
-        indirectionTableRead: Option<BC.ReqId>)
-    | Unready
 
   datatype Variables = Variables(
     bc: BCVariables,
     jc: CommitterModel.CM)
-
-  // datatype Sector =
-  //   | SectorNode(node: Node)
-  //   | SectorIndirectionTable(indirectionTable: IndirectionTable)
-  //   | SectorSuperblock(superblock: SectorType.Superblock)
-
-  predicate IsLocAllocIndirectionTable(indirectionTable: IndirectionTable, i: int)
-  {
-    IndirectionTableModel.IsLocAllocIndirectionTable(indirectionTable, i)
-  }
-
-  predicate IsLocAllocOutstanding(outstanding: map<BC.ReqId, BC.OutstandingWrite>, i: int)
-  {
-    !(forall id | id in outstanding :: outstanding[id].loc.addr as int != i * NodeBlockSize() as int)
-  }
-
-  predicate IsLocAllocBitmap(bm: BitmapModel.BitmapModelT, i: int)
-  {
-    IndirectionTableModel.IsLocAllocBitmap(bm, i)
-  }
-
-  predicate {:opaque} ConsistentBitmap(
-      ephemeralIndirectionTable: IndirectionTable,
-      frozenIndirectionTable: Option<IndirectionTable>,
-      persistentIndirectionTable: IndirectionTable,
-      outstandingBlockWrites: map<BC.ReqId, BC.OutstandingWrite>,
-      blockAllocator: BlockAllocatorModel.BlockAllocatorModel)
-  {
-    && (forall i: int :: IsLocAllocIndirectionTable(ephemeralIndirectionTable, i)
-      <==> IsLocAllocBitmap(blockAllocator.ephemeral, i))
-    && (forall i: int :: IsLocAllocIndirectionTable(persistentIndirectionTable, i)
-      <==> IsLocAllocBitmap(blockAllocator.persistent, i))
-    && (frozenIndirectionTable.Some? <==> blockAllocator.frozen.Some?)
-    && (frozenIndirectionTable.Some? ==>
-      (forall i: int :: IsLocAllocIndirectionTable(frozenIndirectionTable.value, i)
-        <==> IsLocAllocBitmap(blockAllocator.frozen.value, i)))
-    && (forall i: int :: IsLocAllocOutstanding(outstandingBlockWrites, i)
-      <==> IsLocAllocBitmap(blockAllocator.outstanding, i))
-  }
-
-  // predicate WFNode(node: Node)
-  // {
-  //   BT.WFNode(node)
-  // }
-
-  predicate WFCache(cache: map<Reference, Node>)
-  {
-    forall ref | ref in cache :: SSM.WFNode(cache[ref])
-  }
-
-  function TotalCacheSize(s: BCVariables) : int
-  requires s.Ready?
-  {
-    |s.cache| + |s.outstandingBlockReads|
-  }
-
-  predicate WFVarsReady(s: BCVariables)
-  requires s.Ready?
-  {
-    var Ready(persistentIndirectionTable, frozenIndirectionTable, ephemeralIndirectionTable, persistentIndirectionTableLoc, frozenIndirectionTableLoc, outstandingIndirectionTableWrite, oustandingBlockWrites, outstandingBlockReads, cache, lru, locBitmap) := s;
-    && WFCache(cache)
-    && LruModel.WF(lru)
-    && LruModel.I(lru) == cache.Keys
-    && TotalCacheSize(s) <= MaxCacheSize()
-    && IndirectionTableModel.Inv(ephemeralIndirectionTable)
-    && IndirectionTableModel.TrackingGarbage(ephemeralIndirectionTable)
-    && IndirectionTableModel.Inv(persistentIndirectionTable)
-    && (frozenIndirectionTable.Some? ==> IndirectionTableModel.Inv(frozenIndirectionTable.value))
-    && BlockAllocatorModel.Inv(s.blockAllocator)
-    && ConsistentBitmap(s.ephemeralIndirectionTable, s.frozenIndirectionTable,
-        s.persistentIndirectionTable, s.outstandingBlockWrites, s.blockAllocator)
-  }
-  predicate WFBCVars(vars: BCVariables)
-  {
-    && (vars.Ready? ==> WFVarsReady(vars))
-  }
-  // predicate WFSector(sector: Sector)
-  // {
-  //   match sector {
-  //     case SectorNode(node) => WFNode(node)
-  //     case SectorIndirectionTable(indirectionTable) => (
-  //       && IndirectionTableModel.Inv(indirectionTable)
-  //       && BC.WFCompleteIndirectionTable(IIndirectionTable(indirectionTable))
-  //     )
-  //     case SectorSuperblock(superblock) =>
-  //       JC.WFSuperblock(superblock)
-  //   }
-  // }
-
-  function INode(node: Node) : (result: BT.G.Node)
-  {
-    BT.G.Node(node.pivotTable, node.children, node.buckets)
-  }
-  function ICache(cache: map<Reference, Node>): map<Reference, BT.G.Node>
-  requires WFCache(cache)
-  {
-    map ref | ref in cache :: INode(cache[ref])
-  }
-  // function IIndirectionTable(table: IndirectionTable) : (result: SectorType.IndirectionTable)
-  // {
-  //   IndirectionTableModel.I(table)
-  // }
-  function IIndirectionTableOpt(table: Option<IndirectionTable>) : (result: Option<SectorType.IndirectionTable>)
-  {
-    if table.Some? then
-      Some(SSM.IIndirectionTable(table.value))
-    else
-      None
-  }
-  function IBlockCache(vars: BCVariables) : BBC.Variables
-  requires WFBCVars(vars)
-  {
-    match vars {
-      case Ready(persistentIndirectionTable, frozenIndirectionTable, ephemeralIndirectionTable, persistentIndirectionTableLoc, frozenIndirectionTableLoc, outstandingIndirectionTableWrite, oustandingBlockWrites, outstandingBlockReads, cache, lru, locBitmap) =>
-        BC.Ready(SSM.IIndirectionTable(persistentIndirectionTable), IIndirectionTableOpt(frozenIndirectionTable), SSM.IIndirectionTable(ephemeralIndirectionTable),  persistentIndirectionTableLoc, frozenIndirectionTableLoc, outstandingIndirectionTableWrite, oustandingBlockWrites, outstandingBlockReads, ICache(cache))
-      case LoadingIndirectionTable(loc, read) =>
-        BC.LoadingIndirectionTable(loc, read)
-      case Unready => BC.Unready
-    }
-  }
-  function ISector(sector: Sector) : SectorType.Sector
-  requires SSM.WFSector(sector)
-  {
-    match sector {
-      case SectorNode(node) => SectorType.SectorNode(INode(node))
-      case SectorIndirectionTable(indirectionTable) => SectorType.SectorIndirectionTable(SSM.IIndirectionTable(indirectionTable))
-      case SectorSuperblock(superblock) => SectorType.SectorSuperblock(superblock)
-    }
-  }
 
   predicate WFVars(s: Variables)
   {
@@ -235,12 +84,6 @@ module StateModel {
   requires WFVars(s)
   {
     IVars(s)
-  }
-
-  predicate BCInv(s: BCVariables)
-  {
-    && WFBCVars(s)
-    && BBC.Inv(IBlockCache(s))
   }
 
   predicate Inv(s: Variables)
