Impl/NodeImpl.i.dfy
@@ -1,6 +1,7 @@
-include "StateModel.i.dfy"
 include "../lib/Buckets/BucketImpl.i.dfy"
 include "../lib/Lang/LinearBox.i.dfy"
+include "../PivotBetree/PivotBetreeSpec.i.dfy"
+include "../lib/DataStructures/MutableMapImpl.i.dfy"
 
 //
 // Implements PivotBetree/PivotBetreeSpec.Node. (There's no Model file
@@ -319,7 +320,6 @@ module BoxNodeImpl {
   import opened BucketWeights
   import opened Options
 
-  import IM = StateModel
   import MM = MutableMap
   import BT = PivotBetreeSpec`Internal
 
