Impl/StateBCModel.i.dfy
@@ -1,0 +1,135 @@
+include "StateSectorModel.i.dfy"
+include "BlockAllocatorModel.i.dfy"
+include "../BlockCacheSystem/BlockJournalDisk.i.dfy"
+include "../BlockCacheSystem/BetreeCache.i.dfy"
+include "../lib/DataStructures/LruModel.i.dfy"
+
+module StateBCModel {
+  import DiskLayout
+  import BitmapModel
+  import BlockAllocatorModel
+
+  import BC = BlockCache
+  import BBC = BetreeCache
+  import LruModel
+  import BT = PivotBetreeSpec`Internal
+  import BJD = BlockJournalDisk
+
+  import opened Options
+  import opened Bounds
+  import opened StateSectorModel
+
+  type Reference = BT.G.Reference
+  type DiskOp = BJD.DiskOp
+
+  datatype BCVariables =
+    | Ready(
+        persistentIndirectionTable: IndirectionTable, // this lets us keep track of available LBAs
+                                                         // TODO replace with something that only tracks LBAs
+        frozenIndirectionTable: Option<IndirectionTable>,
+        ephemeralIndirectionTable: IndirectionTable,
+        persistentIndirectionTableLoc: DiskLayout.Location,
+        frozenIndirectionTableLoc: Option<DiskLayout.Location>,
+        outstandingIndirectionTableWrite: Option<BC.ReqId>,
+        outstandingBlockWrites: map<BC.ReqId, BC.OutstandingWrite>,
+        outstandingBlockReads: map<BC.ReqId, BC.OutstandingRead>,
+        cache: map<Reference, Node>,
+        lru: LruModel.LruQueue,
+        blockAllocator: BlockAllocatorModel.BlockAllocatorModel
+      )
+    | LoadingIndirectionTable(
+        indirectionTableLoc: DiskLayout.Location,
+        indirectionTableRead: Option<BC.ReqId>)
+    | Unready
+
+  function ICache(cache: map<Reference, Node>): map<Reference, BT.G.Node>
+  requires WFCache(cache)
+  {
+    map ref | ref in cache :: INode(cache[ref])
+  }
+
+  function IBlockCache(vars: BCVariables) : BBC.Variables
+  requires WFBCVars(vars)
+  {
+    match vars {
+      case Ready(persistentIndirectionTable, frozenIndirectionTable, ephemeralIndirectionTable, persistentIndirectionTableLoc, frozenIndirectionTableLoc, outstandingIndirectionTableWrite, oustandingBlockWrites, outstandingBlockReads, cache, lru, locBitmap) =>
+        BC.Ready(IIndirectionTable(persistentIndirectionTable), IIndirectionTableOpt(frozenIndirectionTable), IIndirectionTable(ephemeralIndirectionTable),  persistentIndirectionTableLoc, frozenIndirectionTableLoc, outstandingIndirectionTableWrite, oustandingBlockWrites, outstandingBlockReads, ICache(cache))
+      case LoadingIndirectionTable(loc, read) =>
+        BC.LoadingIndirectionTable(loc, read)
+      case Unready => BC.Unready
+    }
+  }
+
+  predicate BCInv(s: BCVariables)
+  {
+    && WFBCVars(s)
+    && BBC.Inv(IBlockCache(s))
+  }
+
+  predicate WFCache(cache: map<Reference, Node>)
+  {
+    forall ref | ref in cache :: WFNode(cache[ref])
+  }
+
+  function TotalCacheSize(s: BCVariables) : int
+  requires s.Ready?
+  {
+    |s.cache| + |s.outstandingBlockReads|
+  }
+
+  predicate IsLocAllocIndirectionTable(indirectionTable: IndirectionTable, i: int)
+  {
+    IndirectionTableModel.IsLocAllocIndirectionTable(indirectionTable, i)
+  }
+
+  predicate IsLocAllocOutstanding(outstanding: map<BC.ReqId, BC.OutstandingWrite>, i: int)
+  {
+    !(forall id | id in outstanding :: outstanding[id].loc.addr as int != i * NodeBlockSize() as int)
+  }
+
+  predicate IsLocAllocBitmap(bm: BitmapModel.BitmapModelT, i: int)
+  {
+    IndirectionTableModel.IsLocAllocBitmap(bm, i)
+  }
+
+  predicate {:opaque} ConsistentBitmap(
+      ephemeralIndirectionTable: IndirectionTable,
+      frozenIndirectionTable: Option<IndirectionTable>,
+      persistentIndirectionTable: IndirectionTable,
+      outstandingBlockWrites: map<BC.ReqId, BC.OutstandingWrite>,
+      blockAllocator: BlockAllocatorModel.BlockAllocatorModel)
+  {
+    && (forall i: int :: IsLocAllocIndirectionTable(ephemeralIndirectionTable, i)
+      <==> IsLocAllocBitmap(blockAllocator.ephemeral, i))
+    && (forall i: int :: IsLocAllocIndirectionTable(persistentIndirectionTable, i)
+      <==> IsLocAllocBitmap(blockAllocator.persistent, i))
+    && (frozenIndirectionTable.Some? <==> blockAllocator.frozen.Some?)
+    && (frozenIndirectionTable.Some? ==>
+      (forall i: int :: IsLocAllocIndirectionTable(frozenIndirectionTable.value, i)
+        <==> IsLocAllocBitmap(blockAllocator.frozen.value, i)))
+    && (forall i: int :: IsLocAllocOutstanding(outstandingBlockWrites, i)
+      <==> IsLocAllocBitmap(blockAllocator.outstanding, i))
+  }
+
+  predicate WFVarsReady(s: BCVariables)
+  requires s.Ready?
+  {
+    var Ready(persistentIndirectionTable, frozenIndirectionTable, ephemeralIndirectionTable, persistentIndirectionTableLoc, frozenIndirectionTableLoc, outstandingIndirectionTableWrite, oustandingBlockWrites, outstandingBlockReads, cache, lru, locBitmap) := s;
+    && WFCache(cache)
+    && LruModel.WF(lru)
+    && LruModel.I(lru) == cache.Keys
+    && TotalCacheSize(s) <= MaxCacheSize()
+    && IndirectionTableModel.Inv(ephemeralIndirectionTable)
+    && IndirectionTableModel.TrackingGarbage(ephemeralIndirectionTable)
+    && IndirectionTableModel.Inv(persistentIndirectionTable)
+    && (frozenIndirectionTable.Some? ==> IndirectionTableModel.Inv(frozenIndirectionTable.value))
+    && BlockAllocatorModel.Inv(s.blockAllocator)
+    && ConsistentBitmap(s.ephemeralIndirectionTable, s.frozenIndirectionTable,
+        s.persistentIndirectionTable, s.outstandingBlockWrites, s.blockAllocator)
+  }
+
+  predicate WFBCVars(vars: BCVariables)
+  {
+    && (vars.Ready? ==> WFVarsReady(vars))
+  }
+}
