Impl/StateSectorImpl.i.dfy
@@ -1,0 +1,78 @@
+include "NodeImpl.i.dfy"
+include "IndirectionTableImpl.i.dfy"
+include "StateSectorModel.i.dfy"
+
+module StateSectorImpl {
+  import opened Options
+  import opened BoxNodeImpl
+  import opened IndirectionTableImpl
+  import JC = JournalCache
+
+  import SectorType
+  import SSM = StateSectorModel
+
+  type MutIndirectionTable = IndirectionTableImpl.IndirectionTable
+  type MutIndirectionTableNullable = IndirectionTableImpl.IndirectionTable?
+
+  datatype Sector =
+    | SectorNode(node: Node)
+    | SectorSuperblock(superblock: SectorType.Superblock)
+    | SectorIndirectionTable(indirectionTable: MutIndirectionTable)
+
+  function SectorObjectSet(sector: Sector) : set<object>
+  {
+    match sector {
+      case SectorIndirectionTable(indirectionTable) => {indirectionTable}
+      case SectorNode(block) => {block}
+      case SectorSuperblock(superblock) => {}
+    }
+  }
+
+  function SectorRepr(sector: Sector) : set<object>
+  reads SectorObjectSet(sector)
+  {
+    match sector {
+      case SectorIndirectionTable(indirectionTable) => {indirectionTable} + indirectionTable.Repr
+      case SectorNode(block) => block.Repr
+      case SectorSuperblock(superblock) => {}
+    }
+  }
+ 
+  function IIndirectionTable(table: MutIndirectionTable) : (result: IndirectionTableModel.IndirectionTable)
+  reads table, table.Repr
+  requires table.Inv()
+  {
+    table.I()
+  }
+ 
+  function IIndirectionTableOpt(table: MutIndirectionTableNullable) : (result: Option<SSM.IndirectionTable>)
+  reads if table != null then {table} + table.Repr else {}
+  requires table != null ==> table.Inv()
+  {
+    if table != null then
+      Some(IIndirectionTable(table))
+    else
+      None
+  }
+
+  predicate WFSector(sector: Sector)
+  reads SectorObjectSet(sector)
+  reads SectorRepr(sector)
+  {
+    && (sector.SectorIndirectionTable? ==> sector.indirectionTable.Inv())
+    && (sector.SectorNode? ==> sector.node.Inv())
+    && (sector.SectorSuperblock? ==> JC.WFSuperblock(sector.superblock))
+  }
+ 
+  function ISector(sector: Sector) : SSM.Sector
+  requires WFSector(sector)
+  reads SectorObjectSet(sector)
+  reads SectorRepr(sector)
+  {
+    match sector {
+      case SectorSuperblock(superblock) => SSM.SectorSuperblock(superblock)
+      case SectorNode(node) => SSM.SectorNode(node.I())
+      case SectorIndirectionTable(indirectionTable) => SSM.SectorIndirectionTable(IIndirectionTable(indirectionTable))
+    }
+  }
+}
